timeprot-subset-invs: Try new kheap-agnostic TA inv def, saves 9 sorries.
I don't have a clear idea if this new `ta_subset_accessible_addrs` as an
inv becomes feasible, but the fact it is kheap-agnostic I would think is
what makes it easier to prove than `ta_subset_accessible_objects`.

If feasible, it obviates the need for the new `no_label_straddling_objs`
invariant we were considering adding as a conjunct to `pas_refined`.

Signed-off-by: Robert Sison <robert.sison@unimelb.edu.au>

proof/infoflow/timeprotection/CachePartitionIntegrity.thy
@@ -118,6 +118,24 @@ definition no_label_straddling_objs :: "'a PAS \<Rightarrow> det_state \<Rightar
        Some ko \<Rightarrow> \<forall>va \<in> obj_addrs ko p. pasObjectAbs aag va = l |
        None \<Rightarrow> True)"
 
+lemma accessible_objs_subset_accessible_addrs:
+  "no_label_straddling_objs aag s \<Longrightarrow>
+   p_footprint (\<Union> (obj_v_footprint s ` policy_accessible_addrs aag (cur_domain s))) \<subseteq>
+   p_footprint (policy_accessible_addrs aag (cur_domain s))"
+  unfolding no_label_straddling_objs_def
+  apply(clarsimp simp:obj_v_footprint_def image_def split:option.splits)
+  apply(rename_tac vas p va)
+  apply(rule_tac x=va in bexI)
+   apply force
+  apply(erule_tac x=p in allE)
+  apply(case_tac "kheap s p")
+   apply force
+  apply clarsimp
+  apply(erule_tac x=va in ballE)
+   apply(force simp:policy_accessible_addrs_def)
+  apply(force simp:policy_accessible_addrs_def)
+  done
+
 \<comment> \<open>That it's sufficient here to prove an invariant that's agnostic of colours, domains, etc.
     rather than proving \<open>owned_objs_well_partitioned\<close> as an invariant directly.\<close>
 lemma owned_addrs_to_objs_well_partitioned:
@@ -182,11 +200,69 @@ lemma owned_to_accessible_objs_well_partitioned:
   apply(force simp:obj_v_footprint_def policy_owned_addrs_def)
   done
 
+\<comment> \<open>Similar to \<open>owned_to_accessible_objs_well_partitioned\<close>, but only about addresses, not objects:
+  If every domain's address is confined to its partition, then all accessible addresses, due to
+  belonging to accessible domains, are confined to the union of those domains' partitions.\<close>
+lemma owned_to_accessible_addrs_well_partitioned:
+  "owned_addrs_well_partitioned aag \<Longrightarrow>
+   all_labels_are_owned aag \<Longrightarrow>
+   accessible_addrs_well_partitioned aag"
+  unfolding accessible_addrs_well_partitioned_def
+  apply clarsimp
+  apply(rename_tac d va)
+  \<comment> \<open>We consider each address \<open>va\<close> that is accessible to, though not necessarily owned by, \<open>d\<close>.
+      We know the L2 partitioning scheme assigns the physical address of \<open>va\<close> to some domain
+        \<open>paddr_L2_domain (addrFromKPPtr va)\<close>
+      But instead of that, we use the domain \<open>d'\<close> determined by the domain assignment
+      (via @{term\<open>pasDomainAbs\<close>}) of \<open>va\<close>'s label (given by @{term\<open>pasObjectAbs\<close>}),
+      which @{term\<open>all_labels_are_owned\<close>} tells us exists.\<close>
+  apply(prop_tac "\<exists>d'. pasObjectAbs aag va \<in> pasDomainAbs aag d'")
+   apply(force simp:all_labels_are_owned_def)
+  apply(clarsimp simp:policy_accessible_partitions_def policy_accessible_domains_def)
+  apply(rename_tac d va d')
+  apply(rule_tac x="domain_L2_partition d'" in exI)
+  apply(rule conjI)
+   apply(rule_tac x=d' in exI)
+   apply clarsimp
+   \<comment> \<open>Note: \<open>va \<in> policy_accessible_addrs aag d\<close> is what tells
+       the intersection of the two sets is nonempty.\<close>
+   apply(erule_tac x=va in in_empty_interE)
+    apply(force simp:policy_owned_addrs_def)
+   apply force
+  \<comment> \<open>We now use @{term\<open>owned_addrs_well_partitioned\<close>} to tell us \<open>va\<close> is in \<open>d'\<close>'s partition.\<close>
+  apply(force simp:owned_addrs_well_partitioned_def policy_owned_addrs_def)
+  done
+
+section \<open> Subset of accessible addresses \<close>
+
 \<comment> \<open>Address subset property: That only the paddrs of policy-accessible labels are ever accessed.\<close>
 definition ta_subset_accessible_addrs :: "'a PAS \<Rightarrow> det_state \<Rightarrow> bool" where
   "ta_subset_accessible_addrs aag s \<equiv>
      p_footprint (touched_addresses' s) \<subseteq>
      p_footprint (policy_accessible_addrs aag (cur_domain s))"
+
+(* If we can prove `ta_subset_accessible_addrs` is invariant directly,
+   then we can obtain `ta_subset_accessible_partitions` without consulting the `kheap` at all. *)
+theorem ta_subset_accessible_addrs_to_partitions:
+  "ta_subset_accessible_addrs aag s \<Longrightarrow>
+   accessible_addrs_well_partitioned aag \<Longrightarrow>
+   ta_subset_accessible_partitions aag s"
+  unfolding ta_subset_accessible_partitions_def ta_subset_accessible_addrs_def
+    accessible_addrs_well_partitioned_def
+  by blast
+
+(* If it's easier to prove `owned_addrs_well_partitioned` than
+   `accessible_addrs_well_partitioned` then we'll additionally need `all_labels_are_owned`.
+   But the impact is questionable - after all, neither of them rely on the state. *)
+lemma ta_subset_accessible_addrs_to_partitions_alternative:
+  "ta_subset_accessible_addrs aag s \<Longrightarrow>
+   all_labels_are_owned aag \<Longrightarrow>
+   owned_addrs_well_partitioned aag \<Longrightarrow>
+   ta_subset_accessible_partitions aag s"
+  by (force intro:ta_subset_accessible_addrs_to_partitions
+    owned_to_accessible_addrs_well_partitioned)
+
+section \<open> Subset of accessible objects \<close>
 
 \<comment> \<open>Object subset property: That only the paddrs of policy-accessible objects are ever accessed.\<close>
 definition ta_subset_accessible_objects :: "'a PAS \<Rightarrow> det_state \<Rightarrow> bool" where
@@ -194,338 +270,302 @@ definition ta_subset_accessible_objects :: "'a PAS \<Rightarrow> det_state \<Rig
      p_footprint (touched_addresses' s) \<subseteq>
      p_footprint (\<Union> (obj_v_footprint s ` policy_accessible_addrs aag (cur_domain s)))"
 
-abbreviation ta_objsubset_inv :: "'a PAS \<Rightarrow> det_state \<Rightarrow> bool" where
-  "ta_objsubset_inv \<equiv> ta_subset_accessible_objects"
-
-(* XXX: Oh. This won't be true because if not every object is allocated to cover the entire
-   of `vas`, then `vas` won't be a subset of its own object footprints. *)
-lemma "no_label_straddling_objs aag s \<Longrightarrow>
-       vas \<subseteq> \<Union> (obj_v_footprint s ` vas)"
-  unfolding no_label_straddling_objs_def obj_v_footprint_def
-  apply(clarsimp split:option.splits)
-  oops
-
-(* XXX: Likewise this is not going to be true for the same reason. *)
-lemma
-  "ta_subset_accessible_addrs aag s \<Longrightarrow> no_label_straddling_objs aag s \<Longrightarrow>
-   ta_subset_accessible_objects aag s"
+(* If it is easier to prove `ta_subset_accessible_objects` than
+   `ta_subset_accessible_addrs` as an invariant,
+   then we need `no_label_straddling_objs` as an invariant too. *)
+lemma ta_subset_accessible_objs_to_addrs:
+  "ta_subset_accessible_objects aag s \<Longrightarrow>
+   no_label_straddling_objs aag s \<Longrightarrow>
+   ta_subset_accessible_addrs aag s"
   unfolding ta_subset_accessible_addrs_def ta_subset_accessible_objects_def
-    no_label_straddling_objs_def
-  apply clarsimp
-  apply(rename_tac va)
-  apply(clarsimp simp:obj_v_footprint_def image_def split:option.splits)
-  apply(erule_tac x=va in allE)
+  using accessible_objs_subset_accessible_addrs
+  by blast
+
+(* Note: If we need it, `no_label_straddling_objs` is the invariant we've discussed
+   adding as a new conjunct of `pas_refined`. *)
+lemma pas_refined_no_label_straddling_objs:
+  "pas_refined aag s \<Longrightarrow> no_label_straddling_objs aag s"
   oops
 
-lemma ta_subset_accessible_partitions':
-  "\<lbrakk>accessible_objs_well_partitioned aag s; ta_subset_accessible_objects aag s\<rbrakk> \<Longrightarrow>
+(* This is one potential way to get from `ta_subset_accessible_objects` to
+   `ta_subset_accessible_partitions`.
+   But we wouldn't want to prove `accessible_objs_well_partitioned` invariant directly
+   because it depends on the state of the `kheap`. *)
+lemma ta_subset_accessible_objs_to_partitions_HARD:
+  "ta_subset_accessible_objects aag s \<Longrightarrow>
+   accessible_objs_well_partitioned aag s \<Longrightarrow>
    ta_subset_accessible_partitions aag s"
   unfolding ta_subset_accessible_partitions_def ta_subset_accessible_objects_def
     accessible_objs_well_partitioned_def
   by blast
 
-(* XXX: So it turns out we don't even need accessible_objs_well_partitioned...
-   we just needed accessible_addrs_well_partitioned and ta_subset_accessible_addrs after all. *)
-lemma ta_subset_accessible_partitions'':
-  "\<lbrakk>accessible_addrs_well_partitioned aag; ta_subset_accessible_addrs aag s\<rbrakk> \<Longrightarrow>
+(* We can avoid proving `accessible_objs_well_partitioned` (which depends on the kheap)
+   if it's straightforward enough to prove `accessible_addrs_well_partitioned`,
+   but in exchange we need to prove `no_label_straddling_objs`. *)
+theorem ta_subset_accessible_objs_to_partitions:
+  "ta_subset_accessible_objects aag s \<Longrightarrow>
+   no_label_straddling_objs aag s \<Longrightarrow>
+   accessible_addrs_well_partitioned aag \<Longrightarrow>
    ta_subset_accessible_partitions aag s"
-  unfolding ta_subset_accessible_partitions_def ta_subset_accessible_addrs_def
-    accessible_addrs_well_partitioned_def
-  by blast
+  apply(drule ta_subset_accessible_objs_to_addrs)
+   apply force
+  apply(drule ta_subset_accessible_addrs_to_partitions)
+   apply force
+  apply force
+  done
 
-(* We expect to add no_label_straddling_objs as a new conjunct of pas_refined *)
-lemma pas_refined_no_label_straddling_objs:
-  "pas_refined aag s \<Longrightarrow> no_label_straddling_objs aag s"
-  oops
-
-theorem ta_subset_accessible_partitions:
-  "\<lbrakk>all_labels_are_owned aag; owned_addrs_well_partitioned aag;
-    no_label_straddling_objs aag s; ta_subset_accessible_objects aag s\<rbrakk> \<Longrightarrow>
+(* Finally, if it's easier to prove `owned_addrs_well_partitioned` than
+   `accessible_addrs_well_partitioned` then we'll additionally need `all_labels_are_owned`.
+   Though, again, the difference in difficulty between the two is questionable because
+   neither of them depend on the state anyway. *)
+lemma ta_subset_accessible_objs_to_partitions_alternative:
+  "ta_subset_accessible_objects aag s \<Longrightarrow>
+   no_label_straddling_objs aag s \<Longrightarrow>
+   all_labels_are_owned aag \<Longrightarrow>
+   owned_addrs_well_partitioned aag \<Longrightarrow>
    ta_subset_accessible_partitions aag s"
-  by (force intro:ta_subset_accessible_partitions'
+  by (force intro:ta_subset_accessible_objs_to_partitions_HARD
     owned_addrs_to_objs_well_partitioned owned_to_accessible_objs_well_partitioned)
 
-\<comment> \<open>Proofs over seL4 kernel that objects never straddle the addresses of distinct labels\<close>
+\<comment> \<open>Proofs of TA subset invariance over seL4 kernel\<close>
 
-lemma owned_objs_well_partitioned_inv:
-  "call_kernel ev \<lbrace>no_label_straddling_objs aag\<rbrace>"
-  sorry
-
-\<comment> \<open>Proofs of accessible-object subset invariance over seL4 kernel\<close>
+abbreviation ta_subset_inv :: "'a PAS \<Rightarrow> det_state \<Rightarrow> bool" where
+  "ta_subset_inv \<equiv> ta_subset_accessible_addrs"
 
 (* For check_active_irq_if *)
 
-lemma do_machine_op_ta_objsubset_inv:
-  "do_machine_op mop \<lbrace>ta_objsubset_inv aag\<rbrace>"
+lemma do_machine_op_ta_subset_inv:
+  "do_machine_op mop \<lbrace>ta_subset_inv aag\<rbrace>"
   sorry
 
 (* For kernel_entry_if *)
 
-lemma set_object_ta_objsubset_inv:
-  "set_object ptr obj \<lbrace>ta_objsubset_inv aag\<rbrace>"
+lemma set_object_ta_subset_inv:
+  "set_object ptr obj \<lbrace>ta_subset_inv aag\<rbrace>"
   sorry
 
-lemma syscall_ta_objsubset_inv:
-  "syscall m_fault h_fault m_error h_error m_finalise \<lbrace>ta_objsubset_inv aag\<rbrace>"
+lemma syscall_ta_subset_inv:
+  "syscall m_fault h_fault m_error h_error m_finalise \<lbrace>ta_subset_inv aag\<rbrace>"
   sorry
 
-lemma resolve_address_bits'_ta_objsubset_inv:
-  "resolve_address_bits' z capcref \<lbrace>ta_objsubset_inv aag\<rbrace>"
+lemma resolve_address_bits'_ta_subset_inv:
+  "resolve_address_bits' z capcref \<lbrace>ta_subset_inv aag\<rbrace>"
   sorry
 
-lemma transfer_caps_loop_ta_objsubset_inv:
-  "transfer_caps_loop ep rcv_buffer n caps slots mi \<lbrace>ta_objsubset_inv aag\<rbrace>"
+lemma lookup_extra_caps_ta_subset_inv:
+  "lookup_extra_caps thread buffer mi \<lbrace>ta_subset_inv aag\<rbrace>"
   sorry
 
-lemma lookup_extra_caps_ta_objsubset_inv:
-  "lookup_extra_caps thread buffer mi \<lbrace>ta_objsubset_inv aag\<rbrace>"
+lemma set_thread_state_ta_subset_inv:
+  "set_thread_state ref ts \<lbrace>ta_subset_inv aag\<rbrace>"
   sorry
 
-lemma get_receive_slots_ta_objsubset_inv:
-  "get_receive_slots thread bufopt \<lbrace>ta_objsubset_inv aag\<rbrace>"
+lemma get_receive_slots_ta_subset_inv:
+  "get_receive_slots thread bufopt \<lbrace>ta_subset_inv aag\<rbrace>"
   sorry
 
-lemma cap_insert_ta_objsubset_inv:
-  "cap_insert new_cap src_slot dest_slot \<lbrace>ta_objsubset_inv aag\<rbrace>"
+lemma set_cdt_ta_subset_inv:
+  "set_cdt t \<lbrace>ta_subset_inv aag\<rbrace>"
   sorry
 
-lemma set_mrs_ta_objsubset_inv:
-  "set_mrs thread buf msgs \<lbrace>ta_objsubset_inv aag\<rbrace>"
+lemma set_original_ta_subset_inv:
+  "set_original slot v \<lbrace>ta_subset_inv aag\<rbrace>"
   sorry
 
-lemma send_fault_ipc_ta_objsubset_inv:
-  "send_fault_ipc tptr fault \<lbrace>ta_objsubset_inv aag\<rbrace>"
+lemma cap_insert_ta_subset_inv:
+  "cap_insert new_cap src_slot dest_slot \<lbrace>ta_subset_inv aag\<rbrace>"
   sorry
 
-lemma decode_read_registers_ta_objsubset_inv:
-  "decode_read_registers data cap \<lbrace>ta_objsubset_inv aag\<rbrace>"
+lemma transfer_caps_loop_ta_subset_inv:
+  "transfer_caps_loop ep rcv_buffer n caps slots mi \<lbrace>ta_subset_inv aag\<rbrace>"
   sorry
 
-lemma lookup_slot_for_cnode_op_ta_objsubset_inv:
-  "lookup_slot_for_cnode_op is_source croot ptr depth \<lbrace>ta_objsubset_inv aag\<rbrace>"
+lemma send_ipc_ta_subset_inv:
+  "send_ipc block call badge can_grant can_grant_reply thread epptr \<lbrace>ta_subset_inv aag\<rbrace>"
   sorry
 
-lemma decode_copy_registers_ta_objsubset_inv:
-  "decode_copy_registers data cap extra_caps \<lbrace>ta_objsubset_inv aag\<rbrace>"
+lemma decode_read_registers_ta_subset_inv:
+  "decode_read_registers data cap \<lbrace>ta_subset_inv aag\<rbrace>"
   sorry
 
-lemma decode_set_tls_base_ta_objsubset_inv:
-  "decode_set_tls_base args cap \<lbrace>ta_objsubset_inv aag\<rbrace>"
+lemma decode_write_registers_ta_subset_inv:
+  "decode_write_registers data cap \<lbrace>ta_subset_inv aag\<rbrace>"
   sorry
 
-lemma decode_write_registers_ta_objsubset_inv:
-  "decode_write_registers data cap \<lbrace>ta_objsubset_inv aag\<rbrace>"
+lemma decode_copy_registers_ta_subset_inv:
+  "decode_copy_registers data cap extra_caps \<lbrace>ta_subset_inv aag\<rbrace>"
   sorry
 
-lemma arch_decode_irq_control_invocation_ta_objsubset_inv:
-  "arch_decode_irq_control_invocation label args src_slot cps \<lbrace>ta_objsubset_inv aag\<rbrace>"
+lemma send_fault_ipc_ta_subset_inv:
+  "send_fault_ipc tptr fault \<lbrace>ta_subset_inv aag\<rbrace>"
   sorry
 
-lemma decode_irq_control_invocation_ta_objsubset_inv:
-  "decode_irq_control_invocation label args src_slot cps \<lbrace>ta_objsubset_inv aag\<rbrace>"
+lemma decode_invocation_ta_subset_inv:
+  "decode_invocation label args cap_index slot cap excaps \<lbrace>ta_subset_inv aag\<rbrace>"
   sorry
 
-lemma decode_asid_control_invocation_ta_objsubset_inv:
-  "decode_asid_control_invocation  label args cte cap extra_caps \<lbrace>ta_objsubset_inv aag\<rbrace>"
+lemma delete_objects_ta_subset_inv:
+  "delete_objects ptr bits \<lbrace>ta_subset_inv aag\<rbrace>"
   sorry
 
-lemma delete_objects_ta_objsubset_inv:
-  "delete_objects ptr bits \<lbrace>ta_objsubset_inv aag\<rbrace>"
+lemma reset_untyped_cap_ta_subset_inv:
+  "reset_untyped_cap src_slot \<lbrace>ta_subset_inv aag\<rbrace>"
   sorry
 
-lemma reset_untyped_cap_ta_objsubset_inv:
-  "reset_untyped_cap src_slot \<lbrace>ta_objsubset_inv aag\<rbrace>"
+lemma retype_region_ta_subset_inv:
+  "retype_region ptr numObjects o_bits type dev \<lbrace>ta_subset_inv aag\<rbrace>"
   sorry
 
-lemma retype_region_ta_objsubset_inv:
-  "retype_region ptr numObjects o_bits type dev \<lbrace>ta_objsubset_inv aag\<rbrace>"
+lemma create_cap_ta_subset_inv:
+  "create_cap type bits untyped is_device dest_oref \<lbrace>ta_subset_inv aag\<rbrace>"
   sorry
 
-lemma create_cap_ta_objsubset_inv:
-  "create_cap type bits untyped is_device dest_oref \<lbrace>ta_objsubset_inv aag\<rbrace>"
+lemma invoke_untyped_ta_subset_inv:
+  "invoke_untyped ui \<lbrace>ta_subset_inv aag\<rbrace>"
   sorry
 
-lemma invoke_untyped_ta_objsubset_inv:
-  "invoke_untyped ui \<lbrace>ta_objsubset_inv aag\<rbrace>"
+lemma cancel_all_ipc_ta_subset_inv:
+  "cancel_all_ipc epptr \<lbrace>ta_subset_inv aag\<rbrace>"
   sorry
 
-lemma decode_invocation_ta_objsubset_inv:
-  "decode_invocation label args cap_index slot cap excaps \<lbrace>ta_objsubset_inv aag\<rbrace>"
+lemma cancel_all_signals_ta_subset_inv:
+  "cancel_all_signals ntftnptr \<lbrace>ta_subset_inv aag\<rbrace>"
   sorry
 
-lemma send_signal_ta_objsubset_inv:
-  "send_signal ntfnptr badge \<lbrace>ta_objsubset_inv aag\<rbrace>"
+lemma set_irq_state_ta_subset_inv:
+  "set_irq_state state irq \<lbrace>ta_subset_inv aag\<rbrace>"
   sorry
 
-lemma suspend_ta_objsubset_inv:
-  "suspend thread \<lbrace>ta_objsubset_inv aag\<rbrace>"
+lemma reply_cancel_ipc_ta_subset_inv:
+  "reply_cancel_ipc tptr \<lbrace>ta_subset_inv aag\<rbrace>"
   sorry
 
-lemma restart_ta_objsubset_inv:
-  "restart thread \<lbrace>ta_objsubset_inv aag\<rbrace>"
+lemma update_waiting_ntfn_ta_subset_inv:
+  "update_waiting_ntfn ntfnptr queue bound_tcb badge \<lbrace>ta_subset_inv aag\<rbrace>"
   sorry
 
-lemma send_ipc_ta_objsubset_inv:
-  "send_ipc block call badge can_grant can_grant_reply thread epptr \<lbrace>ta_objsubset_inv aag\<rbrace>"
+lemma send_signal_ta_subset_inv:
+  "send_signal ntfnptr badge \<lbrace>ta_subset_inv aag\<rbrace>"
   sorry
 
-lemma cap_swap_ta_objsubset_inv:
-  "cap_swap cap1 slot1 cap2 slot2 \<lbrace>ta_objsubset_inv aag\<rbrace>"
+lemma suspend_ta_subset_inv:
+  "suspend thread \<lbrace>ta_subset_inv aag\<rbrace>"
   sorry
 
-lemma empty_slot_ta_objsubset_inv:
-  "empty_slot slot cleanup_info \<lbrace>ta_objsubset_inv aag\<rbrace>"
+lemma restart_ta_subset_inv:
+  "restart thread \<lbrace>ta_subset_inv aag\<rbrace>"
   sorry
 
-lemma delete_asid_pool_ta_objsubset_inv:
-  "delete_asid_pool base ptr \<lbrace>ta_objsubset_inv aag\<rbrace>"
+lemma cap_swap_ta_subset_inv:
+  "cap_swap cap1 slot1 cap2 slot2 \<lbrace>ta_subset_inv aag\<rbrace>"
   sorry
 
-lemma rec_del_ta_objsubset_inv:
-  "rec_del rdc \<lbrace>ta_objsubset_inv aag\<rbrace>"
+lemma empty_slot_ta_subset_inv:
+  "empty_slot slot cleanup_info \<lbrace>ta_subset_inv aag\<rbrace>"
   sorry
 
-lemma check_cap_at_ta_objsubset_inv:
-  "check_cap_at cap slot m \<lbrace>ta_objsubset_inv aag\<rbrace>"
+lemma delete_asid_pool_ta_subset_inv:
+  "delete_asid_pool base ptr \<lbrace>ta_subset_inv aag\<rbrace>"
   sorry
 
-lemma invoke_domain_ta_objsubset_inv:
-  "invoke_domain thread domain \<lbrace>ta_objsubset_inv aag\<rbrace>"
+lemma rec_del_ta_subset_inv:
+  "rec_del rdc \<lbrace>ta_subset_inv aag\<rbrace>"
   sorry
 
-lemma do_reply_transfer_ta_objsubset_inv:
-  "do_reply_transfer sender receiver slot grant  \<lbrace>ta_objsubset_inv aag\<rbrace>"
+lemma check_cap_at_ta_subset_inv:
+  "check_cap_at cap slot m \<lbrace>ta_subset_inv aag\<rbrace>"
   sorry
 
-lemma cap_move_ta_objsubset_inv:
-  "cap_move new_cap src_slot dest_slot \<lbrace>ta_objsubset_inv aag\<rbrace>"
+lemma invoke_domain_ta_subset_inv:
+  "invoke_domain thread domain \<lbrace>ta_subset_inv aag\<rbrace>"
   sorry
 
-lemma cancel_badged_sends_ta_objsubset_inv:
-  "cancel_badged_sends epptr badge \<lbrace>ta_objsubset_inv aag\<rbrace>"
+lemma do_reply_transfer_ta_subset_inv:
+  "do_reply_transfer sender receiver slot grant  \<lbrace>ta_subset_inv aag\<rbrace>"
   sorry
 
-lemma invoke_irq_handler_ta_objsubset_inv:
-  "invoke_irq_handler irqh_invocation \<lbrace>ta_objsubset_inv aag\<rbrace>"
+lemma cap_move_ta_subset_inv:
+  "cap_move new_cap src_slot dest_slot \<lbrace>ta_subset_inv aag\<rbrace>"
   sorry
 
-lemma cap_revoke_ta_objsubset_inv:
-  "cap_revoke slot \<lbrace>ta_objsubset_inv aag\<rbrace>"
+lemma cancel_badged_sends_ta_subset_inv:
+  "cancel_badged_sends epptr badge \<lbrace>ta_subset_inv aag\<rbrace>"
   sorry
 
-lemma perform_asid_control_invocation_ta_objsubset_inv:
-  "perform_asid_control_invocation iv \<lbrace>ta_objsubset_inv aag\<rbrace>"
+lemma invoke_irq_handler_ta_subset_inv:
+  "invoke_irq_handler irqh_invocation \<lbrace>ta_subset_inv aag\<rbrace>"
   sorry
 
-lemma handle_yield_ta_objsubset_inv:
-  "handle_yield \<lbrace>ta_objsubset_inv aag\<rbrace>"
+lemma cap_revoke_ta_subset_inv:
+  "cap_revoke slot \<lbrace>ta_subset_inv aag\<rbrace>"
   sorry
 
-lemma receive_ipc_ta_objsubset_inv:
-  "receive_ipc thread cap is_blocking \<lbrace>ta_objsubset_inv aag\<rbrace>"
+lemma perform_asid_control_invocation_ta_subset_inv:
+  "perform_asid_control_invocation iv \<lbrace>ta_subset_inv aag\<rbrace>"
   sorry
 
-lemma handle_event_ta_objsubset_inv:
-  "handle_event ev \<lbrace>ta_objsubset_inv aag\<rbrace>"
+lemma handle_yield_ta_subset_inv:
+  "handle_yield \<lbrace>ta_subset_inv aag\<rbrace>"
   sorry
 
-lemma invoke_tcb_ta_objsubset_inv:
-  "invoke_tcb iv \<lbrace>ta_objsubset_inv aag\<rbrace>"
+lemma handle_interrupt_ta_subset_inv:
+  "handle_interrupt irq \<lbrace>ta_subset_inv aag\<rbrace>"
   sorry
 
-(* For handle_preemption_if *)
-
-lemma set_thread_state_ta_objsubset_inv:
-  "set_thread_state ref ts \<lbrace>ta_objsubset_inv aag\<rbrace>"
-  sorry
-
-lemma cancel_all_ipc_ta_objsubset_inv:
-  "cancel_all_ipc epptr \<lbrace>ta_objsubset_inv aag\<rbrace>"
-  sorry
-
-lemma set_cdt_ta_objsubset_inv:
-  "set_cdt t \<lbrace>ta_objsubset_inv aag\<rbrace>"
-  sorry
-
-lemma set_original_ta_objsubset_inv:
-  "set_original slot v \<lbrace>ta_objsubset_inv aag\<rbrace>"
-  sorry
-
-lemma set_irq_state_ta_objsubset_inv:
-  "set_irq_state state irq \<lbrace>ta_objsubset_inv aag\<rbrace>"
-  sorry
-
-lemma cancel_all_signals_ta_objsubset_inv:
-  "cancel_all_signals ntftnptr \<lbrace>ta_objsubset_inv aag\<rbrace>"
-  sorry
-
-lemma reply_cancel_ipc_ta_objsubset_inv:
-  "reply_cancel_ipc tptr \<lbrace>ta_objsubset_inv aag\<rbrace>"
-  sorry
-
-lemma update_waiting_ntfn_ta_objsubset_inv:
-  "update_waiting_ntfn ntfnptr queue bound_tcb badge \<lbrace>ta_objsubset_inv aag\<rbrace>"
-  sorry
-
-lemma handle_interrupt_ta_objsubset_inv:
-  "handle_interrupt irq \<lbrace>ta_objsubset_inv aag\<rbrace>"
+lemma handle_event_ta_subset_inv:
+  "handle_event ev \<lbrace>ta_subset_inv aag\<rbrace>"
   sorry
 
 (* For schedule_if *)
 
-lemma switch_to_idle_thread_ta_objsubset_inv:
-  "switch_to_idle_thread \<lbrace>ta_objsubset_inv aag\<rbrace>"
+lemma switch_to_idle_thread_ta_subset_inv:
+  "switch_to_idle_thread \<lbrace>ta_subset_inv aag\<rbrace>"
   sorry
 
-lemma schedule_choose_new_thread_ta_objsubset_inv:
-  "schedule_choose_new_thread \<lbrace>ta_objsubset_inv aag\<rbrace>"
+lemma schedule_choose_new_thread_ta_subset_inv:
+  "schedule_choose_new_thread \<lbrace>ta_subset_inv aag\<rbrace>"
   sorry
 
-lemma switch_to_thread_ta_objsubset_inv:
-  "switch_to_thread t \<lbrace>ta_objsubset_inv aag\<rbrace>"
+lemma switch_to_thread_ta_subset_inv:
+  "switch_to_thread t \<lbrace>ta_subset_inv aag\<rbrace>"
   sorry
 
-lemma schedule_ta_objsubset_inv:
-  "schedule \<lbrace>ta_objsubset_inv aag\<rbrace>"
+lemma schedule_ta_subset_inv:
+  "schedule \<lbrace>ta_subset_inv aag\<rbrace>"
   sorry
 
 \<comment> \<open> Instead of @{term\<open>call_kernel\<close>}, prove for monads used for each step of @{term\<open>ADT_A_if\<close>}. \<close>
 
 crunches check_active_irq_if
-  for ta_objsubset_inv: "ta_objsubset_inv aag"
+  for ta_subset_inv: "ta_subset_inv aag"
   (wp: crunch_wps)
 
-lemma do_user_op_if_ta_objsubset_inv:
-  "do_user_op_if uop tc \<lbrace>ta_objsubset_inv aag\<rbrace>"
+lemma do_user_op_if_ta_subset_inv:
+  "do_user_op_if uop tc \<lbrace>ta_subset_inv aag\<rbrace>"
   sorry
 
 crunches kernel_entry_if
-  for ta_objsubset_inv: "ta_objsubset_inv aag"
+  for ta_subset_inv: "ta_subset_inv aag"
   (wp: crunch_wps simp:crunch_simps)
 
 crunches handle_preemption_if
-  for ta_objsubset_inv: "ta_objsubset_inv aag"
+  for ta_subset_inv: "ta_subset_inv aag"
   (wp: crunch_wps)
 
 crunches schedule_if
-  for ta_objsubset_inv: "ta_objsubset_inv aag"
+  for ta_subset_inv: "ta_subset_inv aag"
   (wp: crunch_wps)
 
 crunches kernel_exit_if
-  for ta_objsubset_inv: "ta_objsubset_inv aag"
+  for ta_subset_inv: "ta_subset_inv aag"
   (wp: crunch_wps)
 
 \<comment> \<open> Now that it's true for the monads of @{term\<open>ADT_A_if\<close>}, seems it's true
      for @{term\<open>call_kernel\<close>} as well. \<close>
 
 crunches call_kernel
-  for ta_objsubset_inv: "ta_objsubset_inv aag"
+  for ta_subset_inv: "ta_subset_inv aag"
   (wp: crunch_wps)
-
-lemma ta_subset_accessible_objects_inv:
-  "call_kernel ev \<lbrace>ta_subset_accessible_objects aag\<rbrace>"
-  using call_kernel_ta_objsubset_inv
-  by blast
 
 end
 
